Kura/Walk/Path.lean
@@ -8,15 +8,15 @@ variable {α β : Type*} {G H : Graph α β} {u v x y z : α} {e e' f g : β} {S
 
 @[mk_iff]
 structure IsPath (G : Graph α β) (W : Walk α β) : Prop where
-  validOn : W.ValidOn G
+  validIn : W.ValidIn G
   nodup : W.vx.Nodup
 
 @[mk_iff]
 structure IsPathFrom (G : Graph α β) (S T : Set α) (W : Walk α β) : Prop where
-  validOn : W.ValidOn G
+  validIn : W.ValidIn G
   nodup : W.vx.Nodup
-  start_mem : W.start ∈ S
-  finish_mem : W.finish ∈ T
+  first_mem : W.first ∈ S
+  last_mem : W.last ∈ T
 
 lemma IsPathFrom.isWalkFrom (h : G.IsPathFrom S T w) : G.IsWalkFrom S T w := sorry
 
@@ -51,8 +51,8 @@ namespace Path
 /-- Create the reverse of a path -/
 def reverse (p : Path α β) : Path α β := ⟨p.val.reverse, by simp [p.prop]⟩
 
-lemma ValidOn.le {p : Path α β} (h : p.val.ValidOn G) (hle : G ≤ H) : p.val.ValidOn H :=
-  Walk.ValidOn.le h hle
+lemma ValidIn.le {p : Path α β} (h : p.val.ValidIn G) (hle : G ≤ H) : p.val.ValidIn H :=
+  Walk.ValidIn.le h hle
 
 lemma of_cons {p : Path α β} (h : p.val = Walk.cons x e w) : w.vx.Nodup := by
   have := h ▸ p.prop
@@ -60,7 +60,7 @@ lemma of_cons {p : Path α β} (h : p.val = Walk.cons x e w) : w.vx.Nodup := by
   exact this.2
 
 lemma of_prefix {p : Path α β} (h : p.val = w1.append w2)
-    (heq : w1.finish = w2.start) : w1.vx.Nodup := by
+    (heq : w1.last = w2.first) : w1.vx.Nodup := by
   have : (w1.append w2).vx = _ ++ _ := append_vx' heq
   rw [← h] at this
   have : w1.vx.Sublist p.val.vx := by
@@ -77,7 +77,7 @@ lemma of_suffix {p : Path α β} (h : p.val = w1.append w2) : w2.vx.Nodup := by
   exact this.nodup p.prop
 
 lemma not_mem_prefix_of_mem_suffix_tail {p : Path α β} (h : p.val = w1 ++ w2)
-    (heq : w1.finish = w2.start) (hmem : u ∈ w2.vx.tail) : u ∉ w1.vx := by
+    (heq : w1.last = w2.first) (hmem : u ∈ w2.vx.tail) : u ∉ w1.vx := by
   have := h ▸ p.prop
   rw [append_vx' heq, nodup_append] at this
   exact (this.2.2 · hmem)
@@ -88,18 +88,18 @@ lemma not_mem_suffix_of_mem_prefix_dropLast {p : Path α β} (h : p.val = w1 ++ 
   rw [append_vx, nodup_append] at this
   exact this.2.2 hmem
 
-lemma eq_start_of_mem_prefix_suffix {p : Path α β} (h : p.val = w1 ++ w2)
-    (heq : w1.finish = w2.start) (hmem1 : u ∈ w1.vx) (hmem2 : u ∈ w2.vx) :
-    u = w2.start := by
+lemma eq_first_of_mem_prefix_suffix {p : Path α β} (h : p.val = w1 ++ w2)
+    (heq : w1.last = w2.first) (hmem1 : u ∈ w1.vx) (hmem2 : u ∈ w2.vx) :
+    u = w2.first := by
   have := h ▸ p.prop
   rw [append_vx' heq, nodup_append] at this
   have := this.2.2 hmem1
-  rw [← w2.vx.head_cons_tail vx_ne_nil, mem_cons, ← start_eq_vx_head] at hmem2
+  rw [← w2.vx.head_cons_tail vx_ne_nil, mem_cons, ← first_eq_vx_head] at hmem2
   simp_all only [imp_false, or_false]
 
-lemma eq_finish_of_mem_prefix_suffix {p : Path α β} (h : p.val = w1 ++ w2)
-    (heq : w1.finish = w2.start) (hmem1 : u ∈ w1.vx) (hmem2 : u ∈ w2.vx) :
-    u = w1.finish := heq ▸ eq_start_of_mem_prefix_suffix h heq hmem1 hmem2
+lemma eq_last_of_mem_prefix_suffix {p : Path α β} (h : p.val = w1 ++ w2)
+    (heq : w1.last = w2.first) (hmem1 : u ∈ w1.vx) (hmem2 : u ∈ w2.vx) :
+    u = w1.last := heq ▸ eq_first_of_mem_prefix_suffix h heq hmem1 hmem2
 
 def append (p q : Path α β) (hDisj : p.val.vx.dropLast.Disjoint q.val.vx) : Path α β :=
   ⟨p.val ++ q.val, by
@@ -108,14 +108,14 @@ def append (p q : Path α β) (hDisj : p.val.vx.dropLast.Disjoint q.val.vx) : Pa
     exact p.prop.sublist (List.dropLast_sublist p.val.vx)⟩
 
 @[simp]
-lemma append_start {p q : Path α β} (heq : p.val.finish = q.val.start)
-    (hDisj : p.val.vx.dropLast.Disjoint q.val.vx) : (p.append q hDisj).val.start = p.val.start :=
-  append_start_of_eq heq
+lemma append_first {p q : Path α β} (heq : p.val.last = q.val.first)
+    (hDisj : p.val.vx.dropLast.Disjoint q.val.vx) : (p.append q hDisj).val.first = p.val.first :=
+  append_first_of_eq heq
 
 @[simp]
-lemma append_finish {p q : Path α β} (hDisj : p.val.vx.dropLast.Disjoint q.val.vx) :
-    (p.append q hDisj).val.finish = q.val.finish := by
-  simp only [append, Walk.append_finish]
+lemma append_last {p q : Path α β} (hDisj : p.val.vx.dropLast.Disjoint q.val.vx) :
+    (p.append q hDisj).val.last = q.val.last := by
+  simp only [append, Walk.append_last]
 
 @[simp]
 lemma append_length {p q : Path α β} (hDisj : p.val.vx.dropLast.Disjoint q.val.vx) :
@@ -133,31 +133,31 @@ lemma append_edge {p q : Path α β} (hDisj : p.val.vx.dropLast.Disjoint q.val.v
   simp only [append, Walk.append_edge]
 
 @[simp]
-lemma append_validOn {p q : Path α β} (heq : p.val.finish = q.val.start)
-    (hpVd : p.val.ValidOn G) (hqVd : q.val.ValidOn G)
-    (hDisj : p.val.vx.dropLast.Disjoint q.val.vx) : (p.append q hDisj).val.ValidOn G :=
-  Walk.append_validOn heq hpVd hqVd
+lemma append_validIn {p q : Path α β} (heq : p.val.last = q.val.first)
+    (hpVd : p.val.ValidIn G) (hqVd : q.val.ValidIn G)
+    (hDisj : p.val.vx.dropLast.Disjoint q.val.vx) : (p.append q hDisj).val.ValidIn G :=
+  Walk.append_validIn heq hpVd hqVd
 
 
 
-lemma edge_not_isLoop {p : Path α β} (he : e ∈ p.val.edge) (hVd : p.val.ValidOn G) : ¬ G.IsLoopAt e x := by
+lemma edge_not_isLoop {p : Path α β} (he : e ∈ p.val.edge) (hVd : p.val.ValidIn G) : ¬ G.IsLoopAt e x := by
   intro hloop
   rw [IsLoopAt_iff_inc₂] at hloop
   obtain ⟨w₁, w₂, hw12, hnin⟩ := eq_append_cons_of_edge_mem he
-  have hbtw' : G.Inc₂ e w₁.finish w₂.start := by
-    simp only [ValidOn, hw12] at hVd
-    obtain ⟨hbtw, H2⟩ := hVd.append_right_validOn
+  have hbtw' : G.Inc₂ e w₁.last w₂.first := by
+    simp only [ValidIn, hw12] at hVd
+    obtain ⟨hbtw, H2⟩ := hVd.append_right_validIn
     exact hbtw
   have hNodup := hw12 ▸ p.prop
   simp only [Walk.append_vx, cons_vx] at hNodup
   have := List.Nodup.of_append_right hNodup
   obtain ⟨rfl, heq⟩ | ⟨rfl, heq⟩ := hloop.eq_or_eq_of_inc₂ hbtw'
-  · rw [← w₂.vx.head_cons_tail vx_ne_nil, heq, start_eq_vx_head] at this
+  · rw [← w₂.vx.head_cons_tail vx_ne_nil, heq, first_eq_vx_head] at this
     simp only [head_cons_tail, nodup_cons, head_mem, not_true_eq_false, false_and] at this
-  · rw [← w₂.vx.head_cons_tail vx_ne_nil, ← heq, start_eq_vx_head] at this
+  · rw [← w₂.vx.head_cons_tail vx_ne_nil, ← heq, first_eq_vx_head] at this
     simp only [head_cons_tail, nodup_cons, head_mem, not_true_eq_false, false_and] at this
 
-lemma ne_of_inc₂_edge_mem (hVd : p.val.ValidOn G) (hbtw : G.Inc₂ e u v)
+lemma ne_of_inc₂_edge_mem (hVd : p.val.ValidIn G) (hbtw : G.Inc₂ e u v)
     (he : e ∈ p.val.edge) : u ≠ v := by
   rintro huv
   refine edge_not_isLoop (x := v) he hVd ?_
@@ -165,38 +165,38 @@ lemma ne_of_inc₂_edge_mem (hVd : p.val.ValidOn G) (hbtw : G.Inc₂ e u v)
   exact huv ▸ hbtw
 
 @[simp]
-lemma start_not_mem_vx_tail {p : Path α β} : p.val.start ∉ p.val.vx.tail := by
+lemma first_not_mem_vx_tail {p : Path α β} : p.val.first ∉ p.val.vx.tail := by
   rintro hmem
   have := p.prop
   rw [← p.val.vx.head_cons_tail vx_ne_nil, List.nodup_cons] at this
-  exact this.1 (start_eq_vx_head ▸ hmem)
+  exact this.1 (first_eq_vx_head ▸ hmem)
 
 @[simp]
-lemma finish_not_mem_vx_dropLast {p : Path α β} : p.val.finish ∉ p.val.vx.dropLast := by
+lemma last_not_mem_vx_dropLast {p : Path α β} : p.val.last ∉ p.val.vx.dropLast := by
   rintro hmem
   have := p.prop
   rw [← p.val.vx.dropLast_append_getLast vx_ne_nil, ← List.concat_eq_append,
     List.nodup_concat] at this
-  exact this.2 (finish_eq_vx_getLast ▸ hmem)
+  exact this.2 (last_eq_vx_getLast ▸ hmem)
 
 @[simp]
-lemma start_eq_finish_iff : p.val.start = p.val.finish ↔ ¬ p.val.Nonempty := by
+lemma first_eq_last_iff : p.val.first = p.val.last ↔ ¬ p.val.Nonempty := by
   obtain ⟨w, hw⟩ := p
-  simp only [start_eq_finish_iff hw, Nonempty.not_iff]
+  simp only [first_eq_last_iff hw, Nonempty.not_iff]
 
 @[simp]
-lemma start_ne_finish_iff : p.val.start ≠ p.val.finish ↔ p.val.Nonempty :=
-  start_eq_finish_iff.not_left
+lemma first_ne_last_iff : p.val.first ≠ p.val.last ↔ p.val.Nonempty :=
+  first_eq_last_iff.not_left
 
 end Path
 
 @[simp]
-lemma Inc₂.path_start (hbtw : G.Inc₂ e u v) (hne : u ≠ v) :
-    (Inc₂.path hbtw hne).val.start = u := by simp only [path, Walk.start]
+lemma Inc₂.path_first (hbtw : G.Inc₂ e u v) (hne : u ≠ v) :
+    (Inc₂.path hbtw hne).val.first = u := by simp only [path, Walk.first]
 
 @[simp]
-lemma Inc₂.path_finish (hbtw : G.Inc₂ e u v) (hne : u ≠ v) :
-    (Inc₂.path hbtw hne).val.finish = v := by simp only [path, Walk.finish]
+lemma Inc₂.path_last (hbtw : G.Inc₂ e u v) (hne : u ≠ v) :
+    (Inc₂.path hbtw hne).val.last = v := by simp only [path, Walk.last]
 
 @[simp]
 lemma Inc₂.path_length (hbtw : G.Inc₂ e u v) (hne : u ≠ v) :
@@ -211,54 +211,37 @@ lemma Inc₂.path_edge (hbtw : G.Inc₂ e u v) (hne : u ≠ v) :
     (Inc₂.path hbtw hne).val.edge = [e] := by simp only [path, Walk.edge]
 
 @[simp]
-lemma Inc₂.path_validOn (hbtw : G.Inc₂ e u v) (hne : u ≠ v) :
-    (Inc₂.path hbtw hne).val.ValidOn G := walk_validOn hbtw
+lemma Inc₂.path_validIn (hbtw : G.Inc₂ e u v) (hne : u ≠ v) :
+    (Inc₂.path hbtw hne).val.ValidIn G := walk_validIn hbtw
 
 @[simp]
-lemma Inc₂.path_validOn' (hbtw : G.Inc₂ e u v) (hne : u ≠ v) :
-    (Inc₂.path hbtw hne).val.ValidOn (G[{u, v}]) := by
-  refine (path_validOn hbtw hne).induce ?_
+lemma Inc₂.path_validIn' (hbtw : G.Inc₂ e u v) (hne : u ≠ v) :
+    (Inc₂.path hbtw hne).val.ValidIn (G[{u, v}]) := by
+  refine (path_validIn hbtw hne).induce ?_
   rintro x hx
   simpa [Inc₂.path] using hx
 
 lemma Connected.iff_path :
-  G.Connected u v ↔ ∃ p : Path α β, p.val.ValidOn G ∧ p.val.start = u ∧ p.val.finish = v := by
+  G.Connected u v ↔ ∃ p : Path α β, p.val.ValidIn G ∧ p.val.first = u ∧ p.val.last = v := by
   classical
   rw [Connected.iff_walk]
   constructor
   · rintro ⟨w, hwVd, rfl, rfl⟩
-    use Path.ofWalk w, dedup_validOn hwVd, dedup_start w, dedup_finish w
+    use Path.ofWalk w, dedup_validIn hwVd, dedup_first w, dedup_last w
   · rintro ⟨p, hpVd, rfl, rfl⟩
     use p.val, hpVd, rfl
 
-lemma Contract.path {α' : Type*} {w : Walk α' β} {p : α → α'} {C : Set β} (hVd : ValidOn G p C)
-    (h : w.ValidOn (G /[p] C)) : ∀ x ∈ G.V, ∀ y ∈ G.V, p x = w.start → p y = w.finish →
-    ∃ p' : Path α β, p'.val.ValidOn G ∧ p'.val.start = x ∧ p'.val.finish = y ∧
+lemma Contract.path {α' : Type*} {w : Walk α' β} {p : α → α'} {C : Set β} (hVd : ValidIn G p C)
+    (h : w.ValidIn (G /[p] C)) : ∀ x ∈ G.V, ∀ y ∈ G.V, p x = w.first → p y = w.last →
+    ∃ p' : Path α β, p'.val.ValidIn G ∧ p'.val.first = x ∧ p'.val.last = y ∧
     {e | e ∈ p'.val.edge} ⊆ {e | e ∈ w.edge ∨ e ∈ C} := by
   classical
   rintro x hx y hy hpx hpy
   obtain ⟨w', hw'Vd, rfl, rfl, hsub⟩ := Contract.walk hVd h x hx y hy hpx hpy
-  use Path.ofWalk w', dedup_validOn hw'Vd, dedup_start w', dedup_finish w',
+  use Path.ofWalk w', dedup_validIn hw'Vd, dedup_first w', dedup_last w',
     Subset.trans (dedup_edge_sublist w') hsub
 
 
 -- /-- If the endpoints of a path are connected in G via a valid path, they are connected in G -/
--- lemma connected_of_validOn (h : p.ValidOn G u v) : G.Connected u v :=
---   Walk.connected_of_validOn h
-
-namespace Path
-section disjoint
-
-/-- A collection of paths is internally disjoint if no vertex appears in more than one path
-  except for the special two vertices u and v. (i.e. the endpoints of the paths. But this is not
-  enforced in the definition) -/
-def InternallyDisjoint (u v : α) (Ps : Set (Path α β)) : Prop :=
-  ∀ x pi pj, pi ∈ Ps → pj ∈ Ps → x ∈ pi.val.vx → x ∈ pj.val.vx → pi ≠ pj → x = u ∨ x = v
-
-/-- A collection of paths is disjoint if no vertex appears in more than one path -/
-def Disjoint (Ps : Set (Path α β)) : Prop :=
-  ∀ x pi pj, pi ∈ Ps → pj ∈ Ps → x ∈ pi.val.vx → x ∈ pj.val.vx → pi = pj
-
-end disjoint
-
-end Path
+-- lemma connected_of_validIn (h : p.ValidIn G u v) : G.Connected u v :=
+--   Walk.connected_of_validIn h
